---
title: "Inverse gamma distribution"
format: html
---

If $X\sim\text{Gamma}(\alpha,\,\beta)$, then the new random variable $Y=1/X$ has the *inverse gamma* distribution. We denote this $Y\sim\text{IG}(\alpha,\,\beta)$. You derived this on [Problem Set 6 #6d](https://sta240-f25.github.io/problems/pset-6.html#problem-6).

## Basic properties


|  |        |
|------|--------------------|
| **Notation** | $X\sim\text{IG}(\alpha,\,\beta)$  |
| **Range** | $(0,\,\infty)$ |
| **Parameter space** | $\alpha,\,\beta>0$ |
| **PDF** | $f(x)=\begin{cases}\frac{\beta^\alpha}{\Gamma(\alpha)}x^{-\alpha-1}e^{-\beta /x} &x> 0\\0 & x\leq0.\end{cases}$ |
| **Expectation** | $\frac{\beta}{\alpha-1}$ if $\alpha>1$ |
| **Variance** | $\frac{\beta^2}{(\alpha-1)^2(\alpha-2)}$ if $\alpha>2$ |




## Derivations

::: {.callout-tip collapse="true"}
## Deriving the density from a change-of-variables


:::

::: {.callout-note collapse="true"}
## General formula for the raw moments

Let $X\sim\text{Gamma}(\alpha,\,\beta)$ and $Y=1/X\sim\text{IG}(\alpha,\,\beta)$. Furthermore, assume $\alpha > k$ for some $k\in\mathbb{N}$. Then the $k$th raw moment of the inverse gamma variate $Y$ is 

$$
\begin{aligned}
E(Y^k)
&=
E\left(\frac{1}{X^k}\right)
\\
&=
\int_0^\infty 
\frac{1}{x^k}
f_X(x)
\,\text{d}x
\\
&=
\int_0^\infty 
\frac{1}{x^k}
\frac{\beta^\alpha}{\Gamma(\alpha)}x^{\alpha-1}e^{-\beta x}
\,\text{d}x
\\
&=
\frac{\beta^\alpha}{\Gamma(\alpha)}
\int_0^\infty 
\underbrace{x^{\alpha-k-1}e^{-\beta x}}_{\text{kernel of Gamma}(\alpha-k,\,\beta)}
\,\text{d}x
\\
&=
\frac{\beta^\alpha}{\Gamma(\alpha)}
\frac{\Gamma(\alpha-k)}{\beta^{\alpha-k}}
\\
&=
\beta^k\frac{\Gamma(\alpha-k)}{\Gamma(\alpha)}.
\end{aligned}
$$

So

$$
\begin{aligned}
E(Y)
&=
\beta\frac{\Gamma(\alpha-1)}{\Gamma(\alpha)}=\beta\frac{\Gamma(\alpha-1)}{\Gamma(\alpha-1+1)}=\beta\frac{\Gamma(\alpha-1)}{(\alpha-1)\Gamma(\alpha-1)}=\frac{\beta}{\alpha-1}
\\
\\
E(Y^2)
&=
\beta^2\frac{\Gamma(\alpha-2)}{\Gamma(\alpha)}
\\
&=
\beta^2\frac{\Gamma(\alpha-2)}{\Gamma(\alpha-1+1)}
\\
&=
\beta^2\frac{\Gamma(\alpha-2)}{(\alpha-1)\Gamma(\alpha-1)}
\\
&=
\beta^2\frac{\Gamma(\alpha-2)}{(\alpha-1)\Gamma(\alpha-2+1)}
\\
&=
\beta^2\frac{\Gamma(\alpha-2)}{(\alpha-1)(\alpha-2)\Gamma(\alpha-2)}
\\
&=
\frac{\beta^2}{(\alpha-1)(\alpha-2)}
\\
\\
\text{var}(Y)
&=
E(Y^2)-E(Y)^2
\\
&=
\frac{\beta^2}{(\alpha-1)(\alpha-2)}
-
\frac{\beta^2}{(\alpha-1)^2}
\\
&=
\beta^2
\left[
\frac{1}{(\alpha-1)(\alpha-2)}
-
\frac{1}{(\alpha-1)^2}
\right]
\\
&=
\beta^2
\frac{\alpha-1-(\alpha-2)}{(\alpha-1)^2(\alpha-2)}
\\
&=
\beta^2
\frac{\alpha-1-\alpha+2}{(\alpha-1)^2(\alpha-2)}
\\
&=
\frac{\beta^2}{(\alpha-1)^2(\alpha-2)}
.
\end{aligned}
$$

:::
